Finish updating rel_expr_lemmas.

veric/expr_rel.v
@@ -6,73 +6,75 @@ Require Import veric.compcert_rmaps.
 Require Import veric.Clight_lemmas.
 Require Export veric.lift.
 Require Export veric.Cop2.
+Require Import veric.tycontext.
 Require Import veric.expr.
 Require Import veric.res_predicates.
 Require Import veric.seplog.
 
-Inductive rel_expr' (rho: environ) (phi: rmap): expr -> val -> Prop :=
+Inductive rel_expr' (Delta: tycontext) (rho: environ) (phi: rmap): expr -> val -> Prop :=
  | rel_expr'_const_int: forall i ty, 
-                 rel_expr' rho phi (Econst_int i ty) (Vint i)
+                 rel_expr' Delta rho phi (Econst_int i ty) (Vint i)
  | rel_expr'_const_float: forall f ty, 
-                 rel_expr' rho phi (Econst_float f ty) (Vfloat f)
+                 rel_expr' Delta rho phi (Econst_float f ty) (Vfloat f)
  | rel_expr'_const_single: forall f ty, 
-                 rel_expr' rho phi (Econst_single f ty) (Vsingle f)
+                 rel_expr' Delta rho phi (Econst_single f ty) (Vsingle f)
  | rel_expr'_const_long: forall i ty, 
-                 rel_expr' rho phi (Econst_long i ty) (Vlong i)
+                 rel_expr' Delta rho phi (Econst_long i ty) (Vlong i)
  | rel_expr'_tempvar: forall id ty v,
                  Map.get (te_of rho) id = Some v ->
-                 rel_expr' rho phi (Etempvar id ty) v
+                 rel_expr' Delta rho phi (Etempvar id ty) v
  | rel_expr'_addrof: forall a ty v,
-                 rel_lvalue' rho phi a v ->
-                 rel_expr' rho phi (Eaddrof a ty) v
+                 rel_lvalue' Delta rho phi a v ->
+                 rel_expr' Delta rho phi (Eaddrof a ty) v
  | rel_expr'_unop: forall a v1 v ty op,
-                 rel_expr' rho phi a v1 ->
+                 rel_expr' Delta rho phi a v1 ->
                  Cop.sem_unary_operation op v1 (typeof a) = Some v ->
-                 rel_expr' rho phi (Eunop op a ty) v
+                 rel_expr' Delta rho phi (Eunop op a ty) v
  | rel_expr'_binop: forall a1 a2 v1 v2 v ty op,
-                 rel_expr' rho phi a1 v1 ->
-                 rel_expr' rho phi a2 v2 ->
-                 (forall m, Cop.sem_binary_operation op v1 (typeof a1) v2 (typeof a2) m = Some v) ->
-                 rel_expr' rho phi (Ebinop op a1 a2 ty) v
+                 rel_expr' Delta rho phi a1 v1 ->
+                 rel_expr' Delta rho phi a2 v2 ->
+                 (forall m, Cop.sem_binary_operation (composite_types Delta) op v1 (typeof a1) v2 (typeof a2) m = Some v) ->
+                 rel_expr' Delta rho phi (Ebinop op a1 a2 ty) v
  | rel_expr'_cast: forall a v1 v ty,
-                 rel_expr' rho phi a v1 ->
+                 rel_expr' Delta rho phi a v1 ->
                  Cop.sem_cast v1 (typeof a) ty = Some v ->
-                 rel_expr' rho phi (Ecast a ty) v
+                 rel_expr' Delta rho phi (Ecast a ty) v
  | rel_expr'_lvalue_By_value: forall a ch sh v1 v2,
                  access_mode (typeof a) = By_value ch ->
-                 rel_lvalue' rho phi a v1 ->
+                 rel_lvalue' Delta rho phi a v1 ->
                  app_pred (mapsto sh (typeof a) v1 v2 * TT ) phi ->
                  v2 <> Vundef ->
-                 rel_expr' rho phi a v2
+                 rel_expr' Delta rho phi a v2
  | rel_expr'_lvalue_By_reference: forall a v1,
                  access_mode (typeof a) = By_reference ->
-                 rel_lvalue' rho phi a v1 ->
-                 rel_expr' rho phi a v1
-with rel_lvalue' (rho: environ) (phi: rmap): expr -> val -> Prop :=
+                 rel_lvalue' Delta rho phi a v1 ->
+                 rel_expr' Delta rho phi a v1
+with rel_lvalue' (Delta: tycontext) (rho: environ) (phi: rmap): expr -> val -> Prop :=
  | rel_expr'_local: forall id ty b,
                  Map.get (ve_of rho) id = Some (b,ty) ->
-                 rel_lvalue' rho phi (Evar id ty) (Vptr  b Int.zero)
+                 rel_lvalue' Delta rho phi (Evar id ty) (Vptr  b Int.zero)
  | rel_expr'_global: forall id ty b,
                  Map.get (ve_of rho) id = None ->
                  Map.get (ge_of rho) id = Some b ->
-                 rel_lvalue' rho phi (Evar id ty) (Vptr b Int.zero)
+                 rel_lvalue' Delta rho phi (Evar id ty) (Vptr b Int.zero)
  | rel_lvalue'_deref: forall a b z ty,
-                 rel_expr' rho phi a (Vptr b z) ->
-                 rel_lvalue' rho phi (Ederef a ty) (Vptr b z)
- | rel_lvalue'_field_struct: forall i ty a b z id fList att delta,
-                 rel_expr' rho phi a (Vptr b z) ->
-                 typeof a = Tstruct id fList att ->
-                 field_offset i fList = Errors.OK delta ->
-                 rel_lvalue' rho phi (Efield a i ty) (Vptr b (Int.add z (Int.repr delta))).
+                 rel_expr' Delta rho phi a (Vptr b z) ->
+                 rel_lvalue' Delta rho phi (Ederef a ty) (Vptr b z)
+ | rel_lvalue'_field_struct: forall i ty a b z id co att delta,
+                 rel_expr' Delta rho phi a (Vptr b z) ->
+                 typeof a = Tstruct id att ->
+                 (composite_types Delta) ! id = Some co ->
+                 field_offset (composite_types Delta) i (co_members co) = Errors.OK delta ->
+                 rel_lvalue' Delta rho phi (Efield a i ty) (Vptr b (Int.add z (Int.repr delta))).
 
 Scheme rel_expr'_sch := Minimality for rel_expr' Sort Prop
   with rel_lvalue'_sch := Minimality for  rel_lvalue' Sort Prop.
 
-Lemma rel_expr'_hered: forall e v rho, hereditary age (fun phi => rel_expr' rho phi e v).
+Lemma rel_expr'_hered: forall Delta e v rho, hereditary age (fun phi => rel_expr' Delta rho phi e v).
 Proof.
 intros.
 intro; intros.
-apply (rel_expr'_sch rho a (rel_expr' rho a') (rel_lvalue' rho a'));
+apply (rel_expr'_sch Delta rho a (rel_expr' Delta rho a') (rel_lvalue' Delta rho a'));
   intros;
   try solve [econstructor; eauto].
   eapply rel_expr'_lvalue_By_value; eauto.
@@ -82,7 +84,7 @@ apply (rel_expr'_sch rho a (rel_expr' rho a') (rel_lvalue' rho a'));
   auto.
 Qed.
 
-Lemma rel_lvalue'_hered: forall e v rho, hereditary age (fun phi => rel_lvalue' rho phi e v).
+Lemma rel_lvalue'_hered: forall Delta e v rho, hereditary age (fun phi => rel_lvalue' Delta rho phi e v).
 Proof.
 intros.
 intro; intros.
@@ -94,34 +96,35 @@ apply rel_expr'_hered with a; auto.
 apply rel_expr'_hered with a; auto.
 Qed.
 
-Program Definition rel_expr (e: expr) (v: val) (rho: environ) : pred rmap :=
-    fun phi => rel_expr' rho phi e v.
+Program Definition rel_expr (Delta: tycontext) (e: expr) (v: val) (rho: environ) : pred rmap :=
+    fun phi => rel_expr' Delta rho phi e v.
 Next Obligation. intros. apply rel_expr'_hered. Defined.
 
-Program Definition rel_lvalue (e: expr) (v: val) (rho: environ) : pred rmap :=
-    fun phi => rel_lvalue' rho phi e v.
+Program Definition rel_lvalue (Delta: tycontext) (e: expr) (v: val) (rho: environ) : pred rmap :=
+    fun phi => rel_lvalue' Delta rho phi e v.
 Next Obligation. intros. apply rel_lvalue'_hered. Defined.
 
 Require Import veric.juicy_mem veric.juicy_mem_lemmas veric.juicy_mem_ops.
 Require Import veric.expr_lemmas.
 
 Lemma rel_expr_relate:
-  forall ge te ve rho e jm v,
+  forall Delta ge te ve rho e jm v,
+           genv_cenv ge = composite_types Delta ->
            rho = construct_rho (filter_genv ge) ve te ->
-           rel_expr e v rho (m_phi jm) ->
+           rel_expr Delta e v rho (m_phi jm) ->
            Clight.eval_expr ge ve te (m_dry jm) e v.
 Proof.
-intros.
+intros until v. intro HH; intros.
 hnf in H0.
-apply (rel_expr'_sch rho (m_phi jm)
+apply (rel_expr'_sch Delta rho (m_phi jm)
      (Clight.eval_expr ge ve te (m_dry jm))
      (fun e v => match v with Vptr b z => Clight.eval_lvalue ge ve te (m_dry jm) e b z
                         | _ => False end));
- intros; subst rho; try solve [econstructor; eauto].
+ intros; subst rho; try solve [econstructor; try rewrite HH; eauto].
 * (* Eaddrof *)
    destruct v0; try contradiction. constructor; auto.
 * (* lvalue *)
-   destruct v1; try contradiction.
+  destruct v1; try contradiction.
   eapply Clight.eval_Elvalue; eauto.
   destruct H4 as [m1 [m2 [? [? _]]]].
   unfold mapsto in H4.
@@ -159,12 +162,13 @@ apply (rel_expr'_sch rho (m_phi jm)
 Qed.
 
 Lemma rel_lvalue_relate:
-  forall ge te ve rho e jm b z,
+  forall Delta ge te ve rho e jm b z,
+           genv_cenv ge = composite_types Delta ->
            rho = construct_rho (filter_genv ge) ve te ->
-           rel_lvalue e (Vptr b z) rho (m_phi jm) ->
+           rel_lvalue Delta e (Vptr b z) rho (m_phi jm) ->
            Clight.eval_lvalue ge ve te (m_dry jm) e b z.
 Proof.
-intros.
+intros until z; intro HH; intros.
 hnf in H0.
 remember (Vptr b z) as v.
 revert b z Heqv; induction H0; subst rho; simpl in *; intros; inv Heqv.
@@ -175,16 +179,9 @@ eapply Clight.eval_Evar_local; auto.
   destruct (type_of_global ge b0) eqn:?; inv H1;
   apply Clight.eval_Evar_global; auto.
 constructor. eapply rel_expr_relate; eauto.
-eapply Clight.eval_Efield_struct; eauto.
+eapply Clight.eval_Efield_struct; try rewrite HH; eauto.
 eapply rel_expr_relate; eauto.
 Qed.
-
-(*
-Transparent Float.singleoffloat.
-Transparent Float.singleofint.
-Transparent Float.singleofintu.
-Transparent Float.single_of_bits.
-*)
 
 Lemma sem_cast_load_result:
  forall v1 t1 t2 v2 ch,
@@ -196,8 +193,8 @@ Proof.
 intros.
 unfold Cop.sem_cast in H0.
 
-destruct t1 as [ | [ | | | ] [ | ] ? | [ | ] ? | [ | ] ? | | | | | | ];
-destruct t2 as [ | [ | | | ] [ | ] ? | [ | ] ? | [ | ] ? | | | | | | ];
+destruct t1 as [ | [ | | | ] [ | ] ? | [ | ] ? | [ | ] ? | | | | | ];
+destruct t2 as [ | [ | | | ] [ | ] ? | [ | ] ? | [ | ] ? | | | | | ];
 inv H; try reflexivity;
  simpl in H0; try discriminate;
  destruct v1; inv H0;
@@ -225,7 +222,7 @@ Lemma deref_loc_load_result:
   Val.load_result ch v2 = v2.
 Proof.
 intros.
-destruct t as [ | [ | | | ] [ | ] ? | [ | ] ? | [ | ] ? | | | | | | ];
+destruct t as [ | [ | | | ] [ | ] ? | [ | ] ? | [ | ] ? | | | | | ];
  inv H0; inversion2 H H1; inv H; unfold Mem.loadv in *;
  apply Mem.load_result in H2; subst; simpl;
  match goal with 
@@ -260,15 +257,15 @@ destruct t as [ | [ | | | ] [ | ] ? | [ | ] ? | [ | ] ? | | | | | | ];
 Qed.
 
 Lemma rel_expr'_fun:
- forall rho phi e v v', rel_expr' rho phi e v -> rel_expr' rho phi e v' -> v=v'.
+ forall Delta rho phi e v v', rel_expr' Delta rho phi e v -> rel_expr' Delta rho phi e v' -> v=v'.
 Proof.
 intros until 1.
-apply (rel_expr'_sch rho phi
-      (fun e v => forall v', rel_expr' rho phi e v -> rel_expr' rho phi e v' -> v=v')
-      (fun e v => forall v', rel_lvalue' rho phi e v -> rel_lvalue' rho phi e v' -> v=v'));
+apply (rel_expr'_sch Delta rho phi
+      (fun e v => forall v', rel_expr' Delta rho phi e v -> rel_expr' Delta rho phi e v' -> v=v')
+      (fun e v => forall v', rel_lvalue' Delta rho phi e v -> rel_lvalue' Delta rho phi e v' -> v=v'));
    auto; intros;
    try match goal with H : _ |- _ => inv H; auto; try congruence end;
-   try match goal with H: rel_lvalue' _ _ _ _ |- _ => solve [inv H] end.
+   try match goal with H: rel_lvalue' _ _ _ _ _ |- _ => solve [inv H] end.
 *
    specialize (H1 _ H0 H9). congruence.
 *
@@ -295,17 +292,17 @@ apply (rel_expr'_sch rho phi
    destruct H9 .
    eapply res_predicates.address_mapsto_fun; split; eauto.
 *
-   specialize (H1 _ H0 H9). congruence.
+   specialize (H1 _ H0 H10). congruence.
 Qed.
 
 Lemma rel_expr_extend:
-  forall e v rho, boxy extendM (rel_expr e v rho).
+  forall Delta e v rho, boxy extendM (rel_expr Delta e v rho).
 Proof.
 intros. apply boxy_i; intros; auto.
 hnf in H0|-*.
-apply (rel_expr'_sch rho w
-      (fun e v => rel_expr' rho w e v -> rel_expr' rho w' e v)
-      (fun e v => rel_lvalue' rho w e v -> rel_lvalue' rho w' e v)); auto; intros;
+apply (rel_expr'_sch Delta rho w
+      (fun e v => rel_expr' Delta rho w e v -> rel_expr' Delta rho w' e v)
+      (fun e v => rel_lvalue' Delta rho w e v -> rel_lvalue' Delta rho w' e v)); auto; intros;
  try solve [match goal with H : _ |- _ => inv H; econstructor; eauto end].
 *
 eapply rel_expr'_lvalue_By_value; eauto.
@@ -319,24 +316,25 @@ eapply rel_expr'_lvalue_By_reference; eauto.
 *
 econstructor 2; eauto.
 *
-inv H5.
-pose proof (rel_expr'_fun _ _ _ _ _ H10 H1). inv H5.
-rewrite H3 in H12. symmetry in H12; inv H12.
-rewrite H4 in H13; symmetry in H13; inv H13.
+inv H6.
+pose proof (rel_expr'_fun _ _ _ _ _ _ H1 H12). inv H6.
+rewrite H3 in H13. symmetry in H13; inv H13.
+rewrite H4 in H14. symmetry in H14; inv H14.
+rewrite H5 in H15; symmetry in H15; inv H15.
 econstructor; eauto.
 Qed.
 
 Lemma rel_lvalue_extend:
-  forall e v rho, boxy extendM (rel_lvalue e v rho).
+  forall Delta e v rho, boxy extendM (rel_lvalue Delta e v rho).
 Proof.
 intros. apply boxy_i; intros; auto.
 hnf in H0|-*.
 inv H0; try solve [econstructor; eauto].
 econstructor 2; eauto.
 econstructor; eauto.
-pose proof (rel_expr_extend a (Vptr b z) rho).
+pose proof (rel_expr_extend Delta a (Vptr b z) rho).
 apply (boxy_e _ _ H0 _ _ H); auto.
 econstructor; eauto.
-apply (boxy_e _ _ (rel_expr_extend a (Vptr b z) rho) _ _ H); auto.
+apply (boxy_e _ _ (rel_expr_extend Delta a (Vptr b z) rho) _ _ H); auto.
 Qed.
 
