progs/nest2.v
@@ -2,61 +2,65 @@ Require Import Clightdefs.
 
 Local Open Scope Z_scope.
 
-Definition _i : ident := 40%positive.
-Definition ___builtin_read32_reversed : ident := 32%positive.
-Definition ___compcert_va_int32 : ident := 16%positive.
-Definition _struct_b : ident := 38%positive.
-Definition ___builtin_fsqrt : ident := 24%positive.
-Definition ___builtin_clz : ident := 22%positive.
-Definition ___compcert_va_int64 : ident := 17%positive.
-Definition ___builtin_memcpy_aligned : ident := 8%positive.
+Definition ___builtin_bswap16 : ident := 40%positive.
+Definition ___i64_udiv : ident := 32%positive.
+Definition ___builtin_annot_intval : ident := 16%positive.
+Definition ___builtin_bswap : ident := 38%positive.
+Definition ___builtin_fmadd : ident := 46%positive.
+Definition _get : ident := 54%positive.
+Definition ___compcert_va_float64 : ident := 24%positive.
+Definition ___compcert_va_int32 : ident := 22%positive.
+Definition ___builtin_membar : ident := 17%positive.
+Definition _x2 : ident := 8%positive.
 Definition ___builtin_subl : ident := 5%positive.
-Definition _main : ident := 43%positive.
-Definition ___builtin_va_start : ident := 12%positive.
-Definition ___builtin_annot_intval : ident := 10%positive.
+Definition ___builtin_read16_reversed : ident := 50%positive.
+Definition ___builtin_fsqrt : ident := 43%positive.
+Definition _b : ident := 12%positive.
+Definition _i : ident := 53%positive.
+Definition ___builtin_fmsub : ident := 47%positive.
+Definition _y1 : ident := 10%positive.
+Definition ___builtin_fmax : ident := 44%positive.
 Definition ___builtin_negl : ident := 3%positive.
 Definition ___builtin_write32_reversed : ident := 2%positive.
 Definition ___builtin_write16_reversed : ident := 1%positive.
-Definition _y2 : ident := 36%positive.
-Definition ___builtin_read16_reversed : ident := 31%positive.
-Definition ___builtin_va_copy : ident := 14%positive.
+Definition ___i64_shr : ident := 36%positive.
+Definition ___i64_sdiv : ident := 31%positive.
+Definition ___builtin_memcpy_aligned : ident := 14%positive.
 Definition ___builtin_mull : ident := 6%positive.
-Definition ___builtin_fmin : ident := 26%positive.
-Definition ___builtin_bswap : ident := 19%positive.
-Definition _p : ident := 39%positive.
-Definition ___builtin_membar : ident := 11%positive.
-Definition _y1 : ident := 37%positive.
+Definition ___i64_dtou : ident := 26%positive.
+Definition ___builtin_va_arg : ident := 19%positive.
+Definition ___builtin_bswap32 : ident := 39%positive.
+Definition _y2 : ident := 11%positive.
+Definition ___builtin_fnmsub : ident := 49%positive.
+Definition ___i64_sar : ident := 37%positive.
 Definition ___builtin_addl : ident := 4%positive.
-Definition ___builtin_fmsub : ident := 28%positive.
-Definition ___builtin_fabs : ident := 7%positive.
-Definition _set : ident := 42%positive.
-Definition ___builtin_bswap16 : ident := 21%positive.
-Definition ___compcert_va_float64 : ident := 18%positive.
-Definition ___builtin_annot : ident := 9%positive.
-Definition _get : ident := 41%positive.
-Definition ___builtin_va_arg : ident := 13%positive.
-Definition ___builtin_fmadd : ident := 27%positive.
-Definition _x2 : ident := 33%positive.
-Definition ___builtin_fmax : ident := 25%positive.
-Definition ___builtin_va_end : ident := 15%positive.
-Definition _x1 : ident := 34%positive.
-Definition ___builtin_fnmadd : ident := 29%positive.
-Definition _struct_a : ident := 35%positive.
-Definition ___builtin_fnmsub : ident := 30%positive.
-Definition ___builtin_ctz : ident := 23%positive.
-Definition ___builtin_bswap32 : ident := 20%positive.
-
-Definition t_struct_a :=
-   (Tstruct _struct_a (Fcons _x1 tdouble (Fcons _x2 tint Fnil)) noattr).
-Definition t_struct_b :=
-   (Tstruct _struct_b
-     (Fcons _y1 tint
-       (Fcons _y2
-         (Tstruct _struct_a (Fcons _x1 tdouble (Fcons _x2 tint Fnil)) noattr)
-         Fnil)) noattr).
+Definition ___i64_utod : ident := 28%positive.
+Definition _x1 : ident := 7%positive.
+Definition ___builtin_ctz : ident := 42%positive.
+Definition ___builtin_va_end : ident := 21%positive.
+Definition ___builtin_va_start : ident := 18%positive.
+Definition _a : ident := 9%positive.
+Definition _p : ident := 52%positive.
+Definition ___builtin_fmin : ident := 45%positive.
+Definition ___builtin_clz : ident := 41%positive.
+Definition ___builtin_fabs : ident := 13%positive.
+Definition ___i64_stod : ident := 27%positive.
+Definition ___i64_smod : ident := 33%positive.
+Definition _main : ident := 56%positive.
+Definition ___i64_dtos : ident := 25%positive.
+Definition ___builtin_annot : ident := 15%positive.
+Definition ___i64_umod : ident := 34%positive.
+Definition ___i64_stof : ident := 29%positive.
+Definition _set : ident := 55%positive.
+Definition ___i64_shl : ident := 35%positive.
+Definition ___i64_utof : ident := 30%positive.
+Definition ___compcert_va_int64 : ident := 23%positive.
+Definition ___builtin_read32_reversed : ident := 51%positive.
+Definition ___builtin_fnmadd : ident := 48%positive.
+Definition ___builtin_va_copy : ident := 20%positive.
 
 Definition v_p := {|
-  gvar_info := t_struct_b;
+  gvar_info := (Tstruct _b noattr);
   gvar_init := (Init_space 16 :: nil);
   gvar_readonly := false;
   gvar_volatile := false
@@ -70,7 +74,9 @@ Definition f_get := {|
   fn_temps := ((_i, tint) :: nil);
   fn_body :=
 (Ssequence
-  (Sset _i (Efield (Efield (Evar _p t_struct_b) _y2 t_struct_a) _x2 tint))
+  (Sset _i
+    (Efield (Efield (Evar _p (Tstruct _b noattr)) _y2 (Tstruct _a noattr))
+      _x2 tint))
   (Sreturn (Some (Etempvar _i tint))))
 |}.
 
@@ -81,8 +87,9 @@ Definition f_set := {|
   fn_vars := nil;
   fn_temps := nil;
   fn_body :=
-(Sassign (Efield (Efield (Evar _p t_struct_b) _y2 t_struct_a) _x2 tint)
-  (Etempvar _i tint))
+(Sassign
+  (Efield (Efield (Evar _p (Tstruct _b noattr)) _y2 (Tstruct _a noattr)) _x2
+    tint) (Etempvar _i tint))
 |}.
 
 Definition f_main := {|
@@ -94,6 +101,12 @@ Definition f_main := {|
   fn_body :=
 Sskip
 |}.
+
+Definition composites : list composite_definition :=
+(Composite _a Struct ((_x1, tdouble) :: (_x2, tint) :: nil) noattr ::
+ Composite _b Struct
+   ((_y1, tint) :: (_y2, (Tstruct _a noattr)) :: nil)
+   noattr :: nil).
 
 Definition prog : Clight.program := {|
 prog_defs :=
@@ -155,6 +168,65 @@ prog_defs :=
                    (mksignature (AST.Tint :: nil) (Some AST.Tfloat)
                      cc_default)) (Tcons (tptr tvoid) Tnil) tdouble
      cc_default)) ::
+ (___i64_dtos,
+   Gfun(External (EF_external ___i64_dtos
+                   (mksignature (AST.Tfloat :: nil) (Some AST.Tlong)
+                     cc_default)) (Tcons tdouble Tnil) tlong cc_default)) ::
+ (___i64_dtou,
+   Gfun(External (EF_external ___i64_dtou
+                   (mksignature (AST.Tfloat :: nil) (Some AST.Tlong)
+                     cc_default)) (Tcons tdouble Tnil) tulong cc_default)) ::
+ (___i64_stod,
+   Gfun(External (EF_external ___i64_stod
+                   (mksignature (AST.Tlong :: nil) (Some AST.Tfloat)
+                     cc_default)) (Tcons tlong Tnil) tdouble cc_default)) ::
+ (___i64_utod,
+   Gfun(External (EF_external ___i64_utod
+                   (mksignature (AST.Tlong :: nil) (Some AST.Tfloat)
+                     cc_default)) (Tcons tulong Tnil) tdouble cc_default)) ::
+ (___i64_stof,
+   Gfun(External (EF_external ___i64_stof
+                   (mksignature (AST.Tlong :: nil) (Some AST.Tsingle)
+                     cc_default)) (Tcons tlong Tnil) tfloat cc_default)) ::
+ (___i64_utof,
+   Gfun(External (EF_external ___i64_utof
+                   (mksignature (AST.Tlong :: nil) (Some AST.Tsingle)
+                     cc_default)) (Tcons tulong Tnil) tfloat cc_default)) ::
+ (___i64_sdiv,
+   Gfun(External (EF_external ___i64_sdiv
+                   (mksignature (AST.Tlong :: AST.Tlong :: nil)
+                     (Some AST.Tlong) cc_default))
+     (Tcons tlong (Tcons tlong Tnil)) tlong cc_default)) ::
+ (___i64_udiv,
+   Gfun(External (EF_external ___i64_udiv
+                   (mksignature (AST.Tlong :: AST.Tlong :: nil)
+                     (Some AST.Tlong) cc_default))
+     (Tcons tulong (Tcons tulong Tnil)) tulong cc_default)) ::
+ (___i64_smod,
+   Gfun(External (EF_external ___i64_smod
+                   (mksignature (AST.Tlong :: AST.Tlong :: nil)
+                     (Some AST.Tlong) cc_default))
+     (Tcons tlong (Tcons tlong Tnil)) tlong cc_default)) ::
+ (___i64_umod,
+   Gfun(External (EF_external ___i64_umod
+                   (mksignature (AST.Tlong :: AST.Tlong :: nil)
+                     (Some AST.Tlong) cc_default))
+     (Tcons tulong (Tcons tulong Tnil)) tulong cc_default)) ::
+ (___i64_shl,
+   Gfun(External (EF_external ___i64_shl
+                   (mksignature (AST.Tlong :: AST.Tint :: nil)
+                     (Some AST.Tlong) cc_default))
+     (Tcons tlong (Tcons tint Tnil)) tlong cc_default)) ::
+ (___i64_shr,
+   Gfun(External (EF_external ___i64_shr
+                   (mksignature (AST.Tlong :: AST.Tint :: nil)
+                     (Some AST.Tlong) cc_default))
+     (Tcons tulong (Tcons tint Tnil)) tulong cc_default)) ::
+ (___i64_sar,
+   Gfun(External (EF_external ___i64_sar
+                   (mksignature (AST.Tlong :: AST.Tint :: nil)
+                     (Some AST.Tlong) cc_default))
+     (Tcons tlong (Tcons tint Tnil)) tlong cc_default)) ::
  (___builtin_bswap,
    Gfun(External (EF_builtin ___builtin_bswap
                    (mksignature (AST.Tint :: nil) (Some AST.Tint) cc_default))
@@ -236,6 +308,23 @@ prog_defs :=
                      cc_default)) (Tcons (tptr tuint) (Tcons tuint Tnil))
      tvoid cc_default)) :: (_p, Gvar v_p) :: (_get, Gfun(Internal f_get)) ::
  (_set, Gfun(Internal f_set)) :: (_main, Gfun(Internal f_main)) :: nil);
-prog_main := _main
+prog_public :=
+(_main :: _set :: _get :: _p :: ___builtin_write32_reversed ::
+ ___builtin_write16_reversed :: ___builtin_read32_reversed ::
+ ___builtin_read16_reversed :: ___builtin_fnmsub :: ___builtin_fnmadd ::
+ ___builtin_fmsub :: ___builtin_fmadd :: ___builtin_fmin ::
+ ___builtin_fmax :: ___builtin_fsqrt :: ___builtin_ctz :: ___builtin_clz ::
+ ___builtin_bswap16 :: ___builtin_bswap32 :: ___builtin_bswap ::
+ ___i64_sar :: ___i64_shr :: ___i64_shl :: ___i64_umod :: ___i64_smod ::
+ ___i64_udiv :: ___i64_sdiv :: ___i64_utof :: ___i64_stof :: ___i64_utod ::
+ ___i64_stod :: ___i64_dtou :: ___i64_dtos :: ___compcert_va_float64 ::
+ ___compcert_va_int64 :: ___compcert_va_int32 :: ___builtin_va_end ::
+ ___builtin_va_copy :: ___builtin_va_arg :: ___builtin_va_start ::
+ ___builtin_membar :: ___builtin_annot_intval :: ___builtin_annot ::
+ ___builtin_memcpy_aligned :: ___builtin_fabs :: nil);
+prog_main := _main;
+prog_types := composites;
+prog_comp_env := make_composite_env composites;
+prog_comp_env_eq := refl_equal _
 |}.
 
